First steps in making everything have a foreign_id: push through basics_*.v

theories/interop/basics_resources.v
@@ -17,10 +17,22 @@ Local Program Instance LstorePGMData : PGMData := {
 Next Obligation. eauto. Qed.
 Next Obligation. done. Qed.
 
+Local Program Instance LlocPGMData : PGMData := {
+  K := lloc;
+  V := lloc_visibility;
+  Fpers := lloc_visibility_fid;
+  Pmap := lloc_map_inj;
+}.
+Next Obligation.
+  intros m1 m2 H1 H2.
+  by eapply lloc_map_mono_inj_backwards.
+Qed.
+Next Obligation. intros ???? []%lookup_empty_Some. Qed.
+
 Class wrapperBasicsGpre `{SI: indexT} Σ := WrapperBasicsGpre {
   wrapperG_lstoreG :> pgmG Σ LstorePGMData;
+  wrapperG_lloc_mapG :> pgmG Σ LlocPGMData;
   wrapperG_addr_lvalG :> ghost_mapG Σ addr lval;
-  wrapperG_lloc_mapG :> ghost_mapG Σ lloc lloc_visibility;
 }.
 
 Class wrapperBasicsG `{SI: indexT} Σ := WrapperBasicsG {
@@ -31,12 +43,12 @@ Class wrapperBasicsG `{SI: indexT} Σ := WrapperBasicsG {
 }.
 
 Definition wrapperBasicsΣ {SI: indexT} : gFunctors :=
-  #[pgmΣ LstorePGMData; ghost_mapΣ addr lval;
-    ghost_mapΣ lloc lloc_visibility].
+  #[pgmΣ LstorePGMData; pgmΣ LlocPGMData; ghost_mapΣ addr lval].
 
 Global Instance subG_wrapperBasicsGpre `{SI: indexT} Σ :
   subG wrapperBasicsΣ Σ → wrapperBasicsGpre Σ.
 Proof. solve_inG. Qed.
+
 
 Section BasicsResources.
 Context `{SI: indexT}.
@@ -44,49 +56,60 @@ Context `{!wrapperBasicsG Σ}.
 
 (* Ghost state for [lloc_map] *)
 
-Definition lloc_own_priv dq (γ : lloc) : iProp Σ :=
-  γ ↪[wrapperG_γχvirt]{dq} LlocPrivate.
+Definition lloc_own_priv dq (γ : lloc) fid : iProp Σ :=
+  γ □↪[wrapperG_γχvirt]{dq} (LlocPrivate fid).
 
 Definition lloc_own_foreign (γ : lloc) (id : nat) : iProp Σ :=
-  γ ↪[wrapperG_γχvirt]□ (LlocForeign id).
+  γ □↪[wrapperG_γχvirt]□ (LlocForeign id).
 
-Definition lloc_own_pub (γ : lloc) (ℓ : loc) : iProp Σ :=
-  γ ↪[wrapperG_γχvirt]□ LlocPublic ℓ.
+Definition lloc_own_pub (γ : lloc) fid (ℓ : loc) : iProp Σ :=
+  γ □↪[wrapperG_γχvirt]□ LlocPublic fid ℓ.
 
-Instance lloc_own_pub_persistent γ ℓ : Persistent (lloc_own_pub γ ℓ).
+Definition lloc_own_fid (γ : lloc) fid : iProp Σ :=
+  γ □↪[wrapperG_γχvirt]= fid.
+
+Instance lloc_own_pub_persistent γ fid ℓ : Persistent (lloc_own_pub γ fid ℓ).
 Proof using. apply _. Qed.
 
 Instance lloc_own_foreign_persistent γ id : Persistent (lloc_own_foreign γ id).
 Proof using. apply _. Qed.
 
-Definition lloc_own_auth (χ : lloc_map) : iProp Σ :=
-  "Hχgmap" ∷ ghost_map_auth wrapperG_γχvirt 1 χ ∗
-  "Hχpubs" ∷ ([∗ map] γ↦ℓ ∈ (lloc_map_pubs χ), lloc_own_pub γ ℓ) ∗
-  "Hχforeign" ∷ ([∗ map] γ↦id ∈ (lloc_map_foreign χ), lloc_own_foreign γ id).
+Instance lloc_own_fid_persistent γ id : Persistent (lloc_own_fid γ id).
+Proof using. apply _. Qed.
 
-Notation "γ ~ℓ~ ℓ" := (lloc_own_pub γ ℓ)
-  (at level 20, format "γ  ~ℓ~  ℓ").
-Notation "γ ~ℓ~/" := (lloc_own_priv (DfracOwn 1) γ)
-  (at level 20, format "γ  ~ℓ~/").
-Notation "γ ~ℓ~/{ dq }" := (lloc_own_priv dq γ)
-  (at level 20, format "γ  ~ℓ~/{ dq }").
+Definition lloc_own_auth (χ : lloc_map) : iProp Σ :=
+  "Hχgmap" ∷ pgm_auth wrapperG_γχvirt 1 χ ∗
+  "Hχpubs" ∷ ([∗ map] γ↦ℓ ∈ (lloc_map_pubs χ), ∃ fid, lloc_own_pub γ fid ℓ) ∗
+  "Hχforeign" ∷ ([∗ map] γ↦id ∈ (lloc_map_foreign χ), lloc_own_foreign γ id) ∗
+  "#Hχpers" ∷ ([∗ map] γ↦id ∈ χ, lloc_own_fid γ (lloc_visibility_fid id)).
+
+Notation "γ ~ℓ~ ℓ @ fid" := (lloc_own_pub γ fid ℓ)
+  (at level 20, format "γ  ~ℓ~  ℓ  @  fid").
+Notation "γ ~ℓ~/ @ fid" := (lloc_own_priv (DfracOwn 1) γ fid)
+  (at level 20, format "γ  ~ℓ~/  @  fid").
+Notation "γ ~ℓ~/{ dq } @ fid" := (lloc_own_priv dq γ fid)
+  (at level 20, format "γ  ~ℓ~/{ dq }  @  fid").
 Notation "γ ~foreign~ id" := (lloc_own_foreign γ id)
   (at level 20, format "γ  ~foreign~  id").
+Notation "γ ~@~ id" := (lloc_own_fid γ id)
+  (at level 20, format "γ  ~@~  id").
 
 Lemma lloc_own_auth_get_pub_all χ :
   lloc_own_auth χ -∗
-  [∗ map] γ↦ℓ ∈ (lloc_map_pubs χ), γ ~ℓ~ ℓ.
+  [∗ map] γ↦ℓ ∈ (lloc_map_pubs χ), ∃ fid, γ ~ℓ~ ℓ @ fid.
 Proof using.
   iNamed 1. iApply "Hχpubs".
 Qed.
 
-Lemma lloc_own_auth_get_pub χ γ ℓ :
-  χ !! γ = Some (LlocPublic ℓ) →
+Lemma lloc_own_auth_get_pub χ γ fid ℓ :
+  χ !! γ = Some (LlocPublic fid ℓ) →
   lloc_own_auth χ -∗
-  γ ~ℓ~ ℓ.
+  γ ~ℓ~ ℓ @ fid.
 Proof using.
   intros Hγ. iNamed 1.
-  iDestruct (big_sepM_lookup with "Hχpubs") as "?"; eauto.
+  iDestruct (big_sepM_lookup with "Hχpubs") as "(%fid'&HH)"; first eauto.
+  iDestruct (pgm_lookup with "Hχgmap HH") as %HH1.
+  rewrite HH1 in Hγ; simplify_eq. done.
 Qed.
 
 Lemma lloc_own_auth_get_foreign χ γ id :
@@ -98,22 +121,32 @@ Proof using.
   iApply (big_sepM_lookup with "Hχforeign"); eauto.
 Qed.
 
-Lemma lloc_own_pub_of χ γ ℓ :
+
+Lemma lloc_own_auth_get_fid χ γ vis :
+  χ !! γ = Some vis →
   lloc_own_auth χ -∗
-  γ ~ℓ~ ℓ -∗
-  ⌜χ !! γ = Some (LlocPublic ℓ)⌝.
+  γ ~@~ (lloc_visibility_fid vis).
 Proof using.
-  iIntros "Hχ Hpub". iNamed "Hχ".
-  by iDestruct (ghost_map_lookup with "Hχgmap Hpub") as %?.
+  intros Hγ. iNamed 1.
+  iDestruct (big_sepM_lookup with "Hχpers") as "$"; first eauto.
 Qed.
 
-Lemma lloc_own_priv_of dq χ γ :
+Lemma lloc_own_pub_of χ γ fid ℓ :
   lloc_own_auth χ -∗
-  γ ~ℓ~/{ dq } -∗
-  ⌜χ !! γ = Some LlocPrivate⌝.
+  γ ~ℓ~ ℓ @ fid -∗
+  ⌜χ !! γ = Some (LlocPublic fid ℓ)⌝.
 Proof using.
   iIntros "Hχ Hpub". iNamed "Hχ".
-  by iDestruct (ghost_map_lookup with "Hχgmap Hpub") as %?.
+  by iDestruct (pgm_lookup with "Hχgmap Hpub") as %?.
+Qed.
+
+Lemma lloc_own_priv_of dq χ γ fid :
+  lloc_own_auth χ -∗
+  γ ~ℓ~/{ dq } @ fid -∗
+  ⌜χ !! γ = Some (LlocPrivate fid)⌝.
+Proof using.
+  iIntros "Hχ Hpub". iNamed "Hχ".
+  by iDestruct (pgm_lookup with "Hχgmap Hpub") as %?.
 Qed.
 
 Lemma lloc_own_foreign_of χ γ id :
@@ -122,83 +155,96 @@ Lemma lloc_own_foreign_of χ γ id :
   ⌜χ !! γ = Some (LlocForeign id)⌝.
 Proof using.
   iIntros "Hχ Hfor". iNamed "Hχ".
-  by iDestruct (ghost_map_lookup with "Hχgmap Hfor") as %?.
+  by iDestruct (pgm_lookup with "Hχgmap Hfor") as %?.
 Qed.
 
-Lemma lloc_own_expose χ γ ℓ :
+Lemma lloc_own_pers_of χ γ id :
   lloc_own_auth χ -∗
-  γ ~ℓ~/ ==∗
-  lloc_own_auth (<[γ:=LlocPublic ℓ]> χ) ∗ γ ~ℓ~ ℓ.
+  γ ~@~ id -∗
+  ⌜∃ vis, id = lloc_visibility_fid vis ∧ χ !! γ = Some vis⌝.
 Proof using.
-  iIntros "Hχ Hγ".
+  iIntros "Hχ Hfor". iNamed "Hχ".
+  by iDestruct (pgm_lookup_pers with "Hχgmap Hfor") as %?.
+Qed.
+
+Lemma lloc_own_expose χ γ ℓ fid :
+  ℓ ∉ lloc_map_pub_locs χ →
+  lloc_own_auth χ -∗
+  γ ~ℓ~/ @ fid ==∗
+  lloc_own_auth (<[γ:=LlocPublic fid ℓ]> χ) ∗ γ ~ℓ~ ℓ @ fid.
+Proof using.
+  iIntros (Hpubs) "Hχ Hγ".
+  unfold lloc_own_priv, lloc_own_auth.
   iDestruct (lloc_own_priv_of with "Hχ Hγ") as %Hχγ.
   iNamed "Hχ".
-  iMod (ghost_map_update with "Hχgmap Hγ") as "[$ Hγ]".
-  iMod (ghost_map_elem_persist with "Hγ") as "#Hγ".
+  iMod (pgm_update (D:=LlocPGMData) (LlocPublic fid ℓ) with "Hχgmap Hγ") as "[$ Hγ]".
+  1: done.
+  1: intros Hinj; by apply expose_llocs_insert.
+  iMod (pgm_elem_persist with "Hγ") as "#Hγ".
+  iPoseProof (pgm_elem_to_pers with "Hγ") as "#Hγpers".
   iFrame "Hγ". iModIntro. rewrite /named.
-  iSplitL "Hχpubs".
+  iSplitL "Hχpubs"; last iSplitL.
   { rewrite lloc_map_pubs_insert_pub.
     iApply big_sepM_insert; eauto.
     apply lloc_map_pubs_lookup_None; eauto. }
   { rewrite lloc_map_foreign_insert_pub delete_notin //.
     destruct (lloc_map_foreign χ !! γ) eqn:Heq; try done.
     apply lloc_map_foreign_lookup_Some in Heq; congruence. }
+  { destruct  (χ !! γ) eqn:Heq.
+    2: by iApply big_sepM_insert.
+    rewrite -insert_delete_insert. cbn.
+    iApply big_sepM_insert. 1: by eapply lookup_delete.
+    cbn.
+    iApply (big_sepM_delete (λ k v, k ~@~ lloc_visibility_fid v) χ γ (LlocPrivate fid)); first by simplify_eq.
+    done. }
 Qed.
 
-Lemma lloc_own_allocate χ γ:
+Lemma lloc_own_allocate χ γ fid:
+  (∀ (γ' : nat) (vis' : lloc_visibility), γ ≠ γ' → χ !! γ' = Some vis' → fid ≠ lloc_visibility_fid vis') →
   ⌜χ !! γ = None⌝ -∗
   lloc_own_auth χ ==∗
-  lloc_own_auth (<[γ:=LlocPrivate]> χ) ∗ γ ~ℓ~/.
+  lloc_own_auth (<[γ:=LlocPrivate fid]> χ) ∗ γ ~ℓ~/ @ fid.
 Proof using.
-  iIntros (Hne) "Hχ".
+  iIntros (Hfresh Hne) "Hχ".
   iNamed "Hχ".
-  iMod (ghost_map_insert with "Hχgmap") as "[Hχmap Hγ]"; first done.
+  iMod (pgm_insert with "Hχgmap") as "[Hχmap Hγ]"; first done.
+  1: intros H; by apply lloc_map_inj_insert_priv.
+  iPoseProof (pgm_elem_to_pers with "Hγ") as "#Hγpers".
   iModIntro. iSplitR "Hγ"; last done.
   iSplitL "Hχmap"; first done. unfold named.
-  iSplitL "Hχpubs".
-  { rewrite lloc_map_pubs_insert_priv delete_notin.
-    2: destruct (lloc_map_pubs χ !! γ) eqn:Heq; try done; apply lloc_map_pubs_lookup_Some in Heq; congruence.
-    done. }
+  iSplitL "Hχpubs"; last iSplitL.
+  { rewrite lloc_map_pubs_insert_priv delete_notin. 1: done.
+    destruct (lloc_map_pubs χ !! γ) eqn:Heq; try done.
+    apply lloc_map_pubs_lookup_Some in Heq as (?&Heq); try congruence. }
   { rewrite lloc_map_foreign_insert_priv delete_notin //.
     destruct (lloc_map_foreign χ !! γ) eqn:Heq; try done.
     apply lloc_map_foreign_lookup_Some in Heq; congruence. }
+  { iApply big_sepM_insert; first done. by iSplit. }
 Qed.
 
 Lemma lloc_own_allocate_foreign χ γ id:
+  (∀ (γ' : nat) (vis' : lloc_visibility), γ ≠ γ' → χ !! γ' = Some vis' → id ≠ lloc_visibility_fid vis') →
   ⌜χ !! γ = None⌝ -∗
   lloc_own_auth χ ==∗
   lloc_own_auth (<[γ:=LlocForeign id]> χ) ∗ γ ~foreign~ id.
 Proof using.
-  iIntros (Hne) "Hχ".
+  iIntros (Hfresh Hne) "Hχ".
   iNamed "Hχ".
-  iMod (ghost_map_insert _ (LlocForeign id) with "Hχgmap") as "[Hχmap Hγ]"; first done.
-  iMod (ghost_map_elem_persist with "Hγ") as "#Hγ".
+  iMod (pgm_insert (D:=LlocPGMData) _ (LlocForeign id) with "Hχgmap") as "[Hχmap Hγ]"; first done.
+  1: intros H; by apply lloc_map_inj_insert_foreign.
+  iMod (pgm_elem_persist with "Hγ") as "#Hγ".
+  iPoseProof (pgm_elem_to_pers with "Hγ") as "#Hγpers".
   iModIntro. iSplitR "Hγ"; last by iApply "Hγ".
   iSplitL "Hχmap"; first done. unfold named.
-  iSplitL "Hχpubs".
+  iSplitL "Hχpubs"; last iSplitL.
   { rewrite lloc_map_pubs_insert_foreign delete_notin.
-    2: destruct (lloc_map_pubs χ !! γ) eqn:Heq; try done; apply lloc_map_pubs_lookup_Some in Heq; congruence.
+    2: destruct (lloc_map_pubs χ !! γ) eqn:Heq; try done; apply lloc_map_pubs_lookup_Some in Heq as (?&Heq); congruence.
     done. }
   { rewrite lloc_map_foreign_insert_foreign.
     iApply big_sepM_insert; eauto.
     destruct (lloc_map_foreign χ !! γ) eqn:Heq; try done.
     apply lloc_map_foreign_lookup_Some in Heq; congruence. }
-Qed.
-
-Lemma lloc_own_insert χ γ v:
-  ⌜χ !! γ = None⌝ -∗
-  lloc_own_auth χ ==∗
-  lloc_own_auth (<[γ:=v]> χ).
-Proof using.
-  iIntros (Hne) "Hχ".
-  destruct v as [l| |].
-  { iMod (lloc_own_allocate with "[] Hχ") as "(Hχ & Hγp)"; first done.
-    iMod (lloc_own_expose with "Hχ Hγp") as "(H & _)".
-    rewrite insert_insert; done. }
-  { iMod (lloc_own_allocate_foreign with "[] Hχ") as "(Hχ & Hγ)"; first done.
-    by iModIntro. }
-  { iMod (lloc_own_allocate with "[] Hχ") as "(Hχ & Hγp)"; first done.
-    by iModIntro. }
+  { iApply big_sepM_insert; first done. by iSplit. }
 Qed.
 
 Lemma lloc_own_mono χ1 χ2 :
@@ -218,25 +264,40 @@ Proof using.
   assert (χ1 !! k = None ∧ χ1 ##ₘ χdiff) as [Hnone Hdisj2] by by apply map_disjoint_insert_r in Hdisj.
   rewrite <- insert_union_r in Hinj; last done.
   iMod (IH with "[Hown]") as "Hown".
-  1: intros i v1 v2 H1 H2; eapply Hinj; (erewrite lookup_insert_ne; first done); intros <-.
-  1-2: apply elem_of_dom_2 in H1,H2; eapply not_elem_of_dom in Hne,Hnone; rewrite dom_union_L in H1,H2; set_solver.
-  1: done.
-  1: done.
-  rewrite <- insert_union_r; last done.
-  iMod (lloc_own_insert with "[] Hown") as "$"; last done.
-  iPureIntro; apply lookup_union_None; done.
+  - eapply lloc_map_mono_inj_backwards. split; last done.
+    apply insert_subseteq. by eapply lookup_union_None.
+  - done.
+  - done.
+  - rewrite <- insert_union_r; last done.
+    destruct v as [fid ℓ|fid|fid].
+    + iMod (lloc_own_allocate with "[] Hown") as "(Hown&Hpriv)".
+      2: iPureIntro; by eapply lookup_union_None.
+      2: iMod (lloc_own_expose with "Hown Hpriv") as "(H&_)".
+      3: by rewrite insert_insert.
+      * intros γ' vis' Hne' Heq1 Heq2.
+        by epose proof (Hinj k γ' _ vis' (ltac:(by rewrite lookup_insert)) (ltac:(by rewrite lookup_insert_ne)) (ltac:(by left))).
+      * intros (fid'&γ'&[(?&?)|(Hne2&HH)]%lookup_insert_Some)%elem_of_lloc_map_pub_locs; first done.
+        eapply Hne2, Hinj.
+        1: by rewrite lookup_insert. 1: by rewrite lookup_insert_ne. right; by eexists.
+    + iMod (lloc_own_allocate_foreign with "[] Hown") as "($&Hforeign)".
+      3: by iModIntro. 2: iPureIntro; by eapply lookup_union_None.
+      intros γ' vis' Hne' Heq1 Heq2.
+      by epose proof (Hinj k γ' _ vis' (ltac:(by rewrite lookup_insert)) (ltac:(by rewrite lookup_insert_ne)) (ltac:(by left))).
+    + iMod (lloc_own_allocate with "[] Hown") as "($&Hpriv)".
+      3: by iModIntro. 2: iPureIntro; by eapply lookup_union_None.
+      intros γ' vis' Hne' Heq1 Heq2.
+      by epose proof (Hinj k γ' _ vis' (ltac:(by rewrite lookup_insert)) (ltac:(by rewrite lookup_insert_ne)) (ltac:(by left))).
 Qed.
 
 (* Ghost state for [lstore] *)
 
 Definition lstore_own_elem (γ : lloc) (dq : dfrac) (b : block) :=
   match mutability b with
-  | Mut => γ □↪[wrapperG_γζvirt]{dq} b
-  | Immut => γ □↪[wrapperG_γζvirt]□ b
+  | Mut => pgm_elem (D:=LstorePGMData) wrapperG_γζvirt γ dq b
+  | Immut => pgm_elem (D:=LstorePGMData) wrapperG_γζvirt γ DfracDiscarded b
   end%I.
 
-Definition lstore_own_head (γ : lloc) (h : block_header) :=  
-  (γ □↪[wrapperG_γζvirt]= h)%I.
+Definition lstore_own_head (γ : lloc) (h : block_header) := pgm_pers (D:=LstorePGMData) wrapperG_γζvirt γ h.
 
 Definition lstore_own_mut (γ : lloc) (dq : dfrac) (b : block) :=
   (lstore_own_elem γ dq b ∗ ⌜mutability b = Mut⌝)%I.
@@ -245,7 +306,7 @@ Definition lstore_own_immut (γ : lloc) (b : block) :=
   (lstore_own_elem γ (DfracOwn 1) b ∗ ⌜mutability b = Immut⌝)%I.
 
 Definition lstore_own_auth (ζ : lstore) : iProp Σ :=
-  "Hζgmap" ∷ pgm_auth wrapperG_γζvirt 1 ζ ∗
+  "Hζgmap" ∷ pgm_auth (D:=LstorePGMData) wrapperG_γζvirt 1 ζ ∗
   "#Hζimmut" ∷ ([∗ map] γ↦b ∈ (lstore_immut_blocks ζ), lstore_own_immut γ b).
 
 Global Instance lstore_own_immut_persistent γ b :
@@ -415,8 +476,8 @@ Definition ismut_of_access (acc : vblock_access) : ismut :=
 Definition lstore_own_vblock γ acc dq b : iProp Σ :=
   lstore_own_elem γ dq (Bvblock (ismut_of_access acc, b)) ∗
   match acc with
-  | F => γ ~ℓ~/
-  | M => ∃ ℓ, γ ~ℓ~ ℓ
+  | F => ∃ fid, γ ~ℓ~/ @ fid
+  | M => ∃ fid ℓ, γ ~ℓ~ ℓ @ fid
   | I => True
   end.
 
@@ -436,7 +497,7 @@ Proof using.
 Qed.
 
 Lemma lstore_own_vblock_M_as_mut γ dq b :
-  lstore_own_vblock γ M dq b ⊣⊢ lstore_own_mut γ dq (Bvblock (Mut, b)) ∗ ∃ ℓ, γ ~ℓ~ ℓ.
+  lstore_own_vblock γ M dq b ⊣⊢ lstore_own_mut γ dq (Bvblock (Mut, b)) ∗ ∃ fid ℓ, γ ~ℓ~ ℓ @ fid.
 Proof using.
   iSplit; unfold lstore_own_vblock.
   { iIntros "(? & H)". iDestruct "H" as (?) "?". iFrame. eauto. }
@@ -444,7 +505,7 @@ Proof using.
 Qed.
 
 Lemma lstore_own_vblock_F_as_mut γ dq b :
-  lstore_own_vblock γ F dq b ⊣⊢ lstore_own_mut γ dq (Bvblock (Mut, b)) ∗ γ ~ℓ~/.
+  lstore_own_vblock γ F dq b ⊣⊢ lstore_own_mut γ dq (Bvblock (Mut, b)) ∗ ∃ fid, γ ~ℓ~/ @ fid.
 Proof using.
   iSplit; unfold lstore_own_vblock.
   { iIntros "[? ?]". by iFrame. }
@@ -455,7 +516,7 @@ Lemma lstore_own_vblock_mutable_as_mut γ dq acc b :
   vblock_access_le M acc →
   lstore_own_vblock γ acc dq b ⊣⊢
   lstore_own_mut γ dq (Bvblock (Mut, b)) ∗
-  match acc with F => γ ~ℓ~/ | M => ∃ ℓ, γ ~ℓ~ ℓ | I => True end.
+  match acc with F => ∃ fid, γ ~ℓ~/ @ fid | M => ∃ fid ℓ, γ ~ℓ~ ℓ @ fid | I => True end.
 Proof using.
   iIntros (Hacc). iSplit.
   { iIntros "[? ?]". iFrame. iSplit; eauto.
@@ -501,8 +562,8 @@ Fixpoint block_sim (v : val) (l : lval) : iProp Σ := match v with
   | ML_lang.LitV (ML_lang.LitInt x) => ⌜l = (Lint x)⌝
   | ML_lang.LitV (ML_lang.LitBool b) => ⌜l = (Lint (if b then 1 else 0))⌝
   | ML_lang.LitV ML_lang.LitUnit => ⌜l = (Lint 0)⌝
-  | ML_lang.LitV (ML_lang.LitLoc ℓ) => ∃ γ, ⌜l = (Lloc γ)⌝ ∗ γ ~ℓ~ ℓ
-  | ML_lang.LitV (ML_lang.LitForeign id) => ∃ γ, ⌜l = (Lloc γ)⌝ ∗ γ ~foreign~ id
+  | ML_lang.LitV (ML_lang.LitLoc ℓ) => ∃ γ fid, ⌜l = (Lloc γ)⌝ ∗ γ ~ℓ~ ℓ @ fid
+  | ML_lang.LitV (ML_lang.LitForeign id) => ∃ γ, ⌜l = (Lloc γ)⌝ ∗ γ ~@~ id
   | ML_lang.PairV v1 v2 => ∃ γ lv1 lv2,
       ⌜l = (Lloc γ)⌝ ∗
       γ ↦imm (TagDefault, [lv1;lv2]) ∗
@@ -541,13 +602,13 @@ Proof using.
   iIntros (Hfreeze Hstorebl Hstore Hdisj H) "Hχ Hζ".
   iDestruct (lstore_own_auth_get_immut_all with "Hζ") as "#Hζimm".
   iInduction H as [] "IH" forall "Hζ Hχ"; cbn; try done.
-  1: iExists γ; iSplit; first done.
+  1: iExists γ, fid; iSplit; first done.
   1: by iApply (lloc_own_auth_get_pub with "Hχ").
   1: iExists γ, lv1, lv2; iSplit; first done; iSplit.
   3-4: iExists γ, lv; iSplit; first done; iSplit.
   7: iExists γ; iSplit; first done.
   8: iExists γ; iSplit; first done.
-  8: by iApply (lloc_own_auth_get_foreign with "Hχ").
+  8: simplify_eq; by iApply (lloc_own_auth_get_fid with "Hχ").
   1,3,5,7:
     try iApply lstore_own_vblock_I_as_imm;
     iApply (big_sepM_lookup with "Hζimm"); try done.
@@ -560,7 +621,7 @@ Proof using.
       apply lookup_union_Some in H as [|]; eauto end.
   all: destruct Hstorebl as [_ Hstorebl2].
   all: specialize (Hstorebl2 γ) as [Hstorebl2 _].
-  all: destruct Hstorebl2 as (ℓ & Vs & Hχ & Hσml); [by eapply elem_of_dom_2|].
+  all: destruct Hstorebl2 as (fid & ℓ & Vs & Hχ & Hσml); [by eapply elem_of_dom_2|].
   all: efeed specialize Hstore; eauto; [eapply lookup_union_Some; by eauto|].
   all: inversion Hstore.
 Qed.
@@ -575,13 +636,13 @@ Proof using.
   iIntros (H) "Hχ Hζ".
   iDestruct (lstore_own_auth_get_immut_all with "Hζ") as "#Hζimm".
   iInduction H as [] "IH" forall "Hζ Hχ"; cbn; try done.
-  1: iExists γ; iSplit; first done.
+  1: iExists γ, fid; iSplit; first done.
   1: by iApply (lloc_own_auth_get_pub with "Hχ").
   1: iExists γ, lv1, lv2; iSplit; first done; iSplit.
   3-4: iExists γ, lv; iSplit; first done; iSplit.
   7: iExists γ; iSplit; first done.
   8: iExists γ; iSplit; first done.
-  8: by iApply (lloc_own_auth_get_foreign with "Hχ").
+  8: simplify_eq; by iApply (lloc_own_auth_get_fid with "Hχ").
   1,3,5,7:
     try iApply lstore_own_vblock_I_as_imm;
     iApply (big_sepM_lookup with "Hζimm"); try done.
@@ -629,19 +690,19 @@ Lemma block_sim_auth_is_val_strong  (ζfreeze ζσ ζvirt ζplus : lstore) (χvi
   ζσ ##ₘ ζvirt →
   lloc_own_auth χvirt -∗
   lstore_own_auth (ζplus ∪ ζvirt) -∗
-  ([∗ map] γ↦b ∈ ζplus, pgm_elem wrapperG_γζvirt γ (DfracOwn 1) b) -∗
+  ([∗ map] γ↦b ∈ ζplus, pgm_elem (D:=LstorePGMData) wrapperG_γζvirt γ (DfracOwn 1) b) -∗
   b ~~ v -∗
   ⌜is_val χvirt ζfreeze v b⌝.
 Proof using.
   iIntros (Hfreeze Hdis) "Hχ Hζ Hplus Hsim".
   iInduction v as [[x|bo| | |]| | | |] "IH" forall (b); cbn.
   all: try (iPure "Hsim" as Hsim; subst; iPureIntro; try econstructor; done).
-  1: {iDestruct "Hsim" as "(%γ & -> & Hsim)".
+  1: {iDestruct "Hsim" as "(%γ & %fid & -> & Hsim)".
       iPoseProof (lloc_own_pub_of with "Hχ Hsim") as "%HH".
       iPureIntro. econstructor. done. }
   1: { iDestruct "Hsim" as "(%γ & -> & Hsim)".
-       iPoseProof (lloc_own_foreign_of with "Hχ Hsim") as "%HH".
-       iPureIntro. econstructor. done. }
+       iDestruct (lloc_own_pers_of with "Hχ Hsim") as %(vis&Heq1&Heq2).
+       iPureIntro. econstructor; done. }
   1: iDestruct "Hsim" as "(%γ & -> & Hsim)".
   2: iDestruct "Hsim" as "(%γ & %lv1 & %lv2 & -> & Hsim & Hlv1 & Hlv2)";
      iPoseProof ("IH" with "Hχ Hζ Hplus Hlv1") as "%Hr1";
@@ -703,7 +764,7 @@ Lemma block_sim_arr_auth_is_val_strong (ζfreeze ζσ ζvirt ζplus : lstore) (�
   ζσ ##ₘ ζvirt →
   lloc_own_auth χvirt -∗
   lstore_own_auth (ζplus ∪ ζvirt) -∗
-  ([∗ map] γ↦b ∈ ζplus, pgm_elem wrapperG_γζvirt γ (DfracOwn 1) b) -∗
+  ([∗ map] γ↦b ∈ ζplus, pgm_elem (D:=LstorePGMData) wrapperG_γζvirt γ (DfracOwn 1) b) -∗
   bb ~~∗ vs -∗
   ⌜Forall2 (is_val χvirt ζfreeze) vs bb⌝.
 Proof using.
@@ -753,14 +814,16 @@ Global Hint Constructors vblock_access_le : core.
 
 (* Re-export notations *)
 
-Notation "γ ~ℓ~ ℓ" := (lloc_own_pub γ ℓ)
-  (at level 20, format "γ  ~ℓ~  ℓ").
-Notation "γ ~ℓ~/{ dq }" := (lloc_own_priv dq γ)
-  (at level 20, format "γ  ~ℓ~/{ dq }").
-Notation "γ ~ℓ~/" := (γ  ~ℓ~/{ DfracOwn 1 })
-  (at level 20, format "γ  ~ℓ~/").
+Notation "γ ~ℓ~ ℓ @ fid" := (lloc_own_pub γ fid ℓ)
+  (at level 20, format "γ  ~ℓ~  ℓ  @  fid").
+Notation "γ ~ℓ~/ @ fid" := (lloc_own_priv (DfracOwn 1) γ fid)
+  (at level 20, format "γ  ~ℓ~/  @  fid").
+Notation "γ ~ℓ~/{ dq } @ fid" := (lloc_own_priv dq γ fid)
+  (at level 20, format "γ  ~ℓ~/{ dq }  @  fid").
 Notation "γ ~foreign~ id" := (lloc_own_foreign γ id)
   (at level 20, format "γ  ~foreign~  id").
+Notation "γ ~@~ id" := (lloc_own_fid γ id)
+  (at level 20, format "γ  ~@~  id").
 
 Notation "lv  ~~  v" := (block_sim v lv) (at level 20).
 Notation "lvs  ~~∗  vs" := (block_sim_arr vs lvs) (at level 20).
